Frap/Exercises/SmallStepImp.lean
@@ -1,0 +1,29 @@
+-- small-step operational semantics for Imp exercises
+
+import Frap.SmallStepImp
+
+namespace CImp
+open Imp
+open AStep
+open BStep
+open CStep
+open Multi
+
+/-
+exercise (3-star)
+-/
+
+theorem par_body_n__Sn' n st
+    : st x = n ∧ st y = 0
+      → Multi CStep (par_loop, st) (par_loop, x !-> n + 1; st) := by
+  sorry
+
+/-
+exercise (3-star)
+-/
+
+theorem par_body_n' n st
+    : st x = 0 ∧ st y = 0
+      → ∃ st', Multi CStep (par_loop, st) (par_loop, st')
+          ∧ st' x = n ∧ st' y = 0 := by
+  sorry
